src/Smallstep.v
@@ -1,3 +1,4 @@
+Require Import CpdtTactics.
 Require Import Closures.
 
 (*
@@ -10,6 +11,7 @@ Require Import Closures.
  *
  * XXX
  * Do we need the order part of compcert's fsim/bsim?
+ * Yes, for fsim->bsim.
  *
  * XXX
  * We should copy over a proof of backward simulation from forward
@@ -28,3 +30,93 @@ Definition bsim_simulation {StateA StateB:Type} (StepA:StateA->StateA->Prop) (St
   forall A1, Match A1 B1 ->
   exists A2, Match A2 B2 /\ plus StepA A1 A2.
 
+
+(* Common infrastructure for nested programs *)
+
+Inductive progstate {R:Type} {P:Type->Type} {S:Type} :=
+  | PS (p:P R) (s:S).
+
+Inductive progreturns {R:Type} {P:Type->Type} {S:Type}
+                      (STEP:@progstate R P S -> @progstate R P S -> Prop)
+                      (RET:R->P R):
+                      P R -> S -> S -> R -> Prop :=
+  | ProgRet: forall (p:P R) (s:S) (s':S) (r:R)
+    (STAR: star STEP (PS p s) (PS (RET r) s')),
+    progreturns STEP RET p s s' r.
+
+Inductive progmatch {R:Type} {P1 P2:Type->Type} {S1 S2:Type}
+                    (COMPILE:P1 R->P2 R)
+                    (MATCH:S1->S2->Prop) :
+                    @progstate R P1 S1 ->
+                    @progstate R P2 S2 -> Prop :=
+  | ProgMatch: forall (p1:P1 R) (p2:P2 R) (s1:S1) (s2:S2)
+    (C: COMPILE p1 = p2)
+    (M: MATCH s1 s2),
+    progmatch COMPILE MATCH (PS p1 s1) (PS p2 s2).
+Hint Constructors progmatch.
+
+
+Module Type SmallStepLang.
+
+Parameter Prog: Type->Type.
+Parameter ReturnOp: forall (R:Type), R->(Prog R).
+Parameter State: Type.
+Parameter Step: forall (R:Type), @progstate R (@Prog) State ->
+                                 @progstate R (@Prog) State -> Prop.
+
+End SmallStepLang.
+
+
+Module Type Refines (L1 L2: SmallStepLang).
+
+Parameter Compile: forall (R:Type), L1.Prog R -> L2.Prog R.
+Parameter StateMatch: L1.State -> L2.State -> Prop.
+Axiom FSim: forall R, forward_simulation (L1.Step R) (L2.Step R).
+
+End Refines.
+
+
+Module RefineSelf (L: SmallStepLang) <: Refines L L.
+
+Definition Compile (R:Type) (p:L.Prog R) := p.
+
+Inductive statematch : L.State -> L.State -> Prop :=
+  | Match: forall s, statematch s s.
+Definition StateMatch := statematch.
+Hint Constructors statematch.
+
+Theorem FSim:
+  forall R,
+  forward_simulation (L.Step R) (L.Step R).
+Proof.
+  intros; exists (@progmatch R L.Prog L.Prog L.State L.State (Compile R) statematch); intros.
+
+  repeat match goal with
+  | [ x: progmatch _ _ _ _ |- _ ] => inversion x; clear x; subst
+  | [ x: statematch _ _ |- _ ] => inversion x; clear x; subst
+  end.
+
+  exists A2; split.
+  - eapply star_step; [ apply H | apply star_refl ].
+  - destruct A2. crush.
+Qed.
+
+End RefineSelf.
+
+
+Module FSimReturn (L1 L2: SmallStepLang)
+                  (Ref12: Refines L1 L2).
+
+(* XXX need to prove that forward simulation implies same return value *)
+
+Theorem fsim_implies_returns:
+  forall (R:Type) p s1 s1' s2 r,
+  progreturns (L1.Step R) (L1.ReturnOp R) p s1 s1' r ->
+  exists s2',
+  progreturns (L2.Step R) (L2.ReturnOp R) (Ref12.Compile R p) s2 s2' r /\
+  Ref12.StateMatch s1' s2'.
+Proof.
+  admit.
+Qed.
+
+End FSimReturn.
